  

# The steps to get a vertex form:
 *Example:*
𝑦=3𝑥²+6𝑥+2
  

## Move the constant to the left side:
𝑦−2=3𝑥²+6𝑥

## Factor the x expressions on the right:
𝑦−2=3(𝑥²+2𝑥)

## Add the square of half the x coefficient to the right, and the corresponding multiple on the left:
𝑦−2+3=3(𝑥²+2𝑥+1)

## Factor out a perfect square binomial:
𝑦+1=3(𝑥+1)²

## Move the constant back to the right side:
𝑦=3(𝑥+1)²−1
𝑦=𝑎(𝑥−𝐡)²+𝐤 

 ## Another way
𝑦 = 𝑎𝑥²+𝑏𝑥+𝑐
𝐡 = −𝑏 / 2𝑎
𝐤 = 𝑎𝐡² + 𝑏𝐡 +𝑐

## Vertex coordinates = (h, k)
(-1,-1)

 
